Unordered shim arrangement (#1)
Executable LockServ with python client

extraction/lockserv/ocaml/LockServArrangement.ml
@@ -1,0 +1,68 @@
+module type IntValue = sig
+  val v : int
+end
+
+module type Params = sig
+  val debug : bool
+  val num_clients : int
+end
+
+module LockServArrangement (P : Params) = struct
+  type name = LockServ.name
+  type state = LockServ.data0
+  type input = LockServ.msg
+  type output = LockServ.msg
+  type msg = LockServ.msg
+  type client_id = int
+  type res = (output list * state) * ((name * msg) list)
+  type task_handler = name -> state -> res
+  type timeout_setter = name -> state -> float
+
+  let systemName = "Lock Server"
+
+  let serializeName = LockServSerialization.serializeName
+
+  let deserializeName = LockServSerialization.deserializeName
+
+  let init = fun n ->
+    let open LockServ in
+    Obj.magic ((lockServ_MultiParams P.num_clients).init_handlers (Obj.magic n))
+
+  let handleIO = fun n i s ->
+    let open LockServ in
+    Obj.magic ((lockServ_MultiParams P.num_clients).input_handlers (Obj.magic n) (Obj.magic i) (Obj.magic s))
+
+  let handleNet = fun dst src m s ->
+    let open LockServ in
+    Obj.magic ((lockServ_MultiParams P.num_clients).net_handlers (Obj.magic dst) (Obj.magic src) (Obj.magic m) (Obj.magic s))
+    
+  let deserializeMsg = LockServSerialization.deserializeMsg
+
+  let serializeMsg = LockServSerialization.serializeMsg
+
+  let deserializeInput = LockServSerialization.deserializeInput
+
+  let serializeOutput = LockServSerialization.serializeOutput
+
+  let debug = P.debug
+
+  let debugInput = fun _ inp ->
+    Printf.printf "[%s] got input %s" (Util.timestamp ()) (LockServSerialization.debugSerializeInput inp);
+    print_newline ()
+
+  let debugRecv = fun _ (nm, msg) ->
+    Printf.printf "[%s] receiving message %s from %s" (Util.timestamp ()) (LockServSerialization.debugSerializeMsg msg) (serializeName nm);
+    print_newline ()
+
+  let debugSend = fun _ (nm, msg) ->
+    Printf.printf "[%s] sending message %s to %s" (Util.timestamp ()) (LockServSerialization.debugSerializeMsg msg) (serializeName nm);
+    print_newline ()
+
+  let createClientId () =
+    let upper_bound = 1073741823 in
+    Random.int upper_bound
+
+  let serializeClientId = string_of_int
+
+  let timeoutTasks = []
+end
