extraction/lockserv/ocaml/LockServSerialization.ml
@@ -1,0 +1,35 @@
+let serializeName : LockServ.name -> string = function
+  | LockServ.Server -> "Server"
+  | LockServ.Client i -> Printf.sprintf "Client-%d" i
+
+let deserializeName (s : string) : LockServ.name option =
+  match s with
+  | "Server" -> Some LockServ.Server
+  | _ -> 
+    try Scanf.sscanf s "Client-%d" (fun x -> Some (LockServ.Client (Obj.magic x)))
+    with _ -> None
+
+let deserializeMsg : string -> LockServ.msg = fun s ->
+  Marshal.from_string s 0
+
+let serializeMsg : LockServ.msg -> string = fun m ->
+  Marshal.to_string m []
+
+let deserializeInput inp c : LockServ.msg option =
+  match inp with
+  | "Unlock" -> Some LockServ.Unlock
+  | "Lock" -> Some (LockServ.Lock c)
+  | "Locked" -> Some (LockServ.Locked c)
+  | _ -> None
+
+let serializeOutput : LockServ.msg -> int * string = function
+  | LockServ.Lock _ -> (0, "Lock") (* never happens *)
+  | LockServ.Unlock -> (0, "Unlock") (* never happens *)
+  | LockServ.Locked c -> (c, "Locked")
+
+let debugSerializeInput : LockServ.msg -> string = function
+  | LockServ.Lock c -> Printf.sprintf "Lock %d" c
+  | LockServ.Unlock -> "Unlock"
+  | LockServ.Locked c -> Printf.sprintf "Locked %d" c
+
+let debugSerializeMsg = debugSerializeInput
