extraction/lockserv/test/SerializationTest.ml
@@ -1,0 +1,32 @@
+open OUnit2
+open ListLabels
+
+let tear_down () test_ctxt = ()
+
+let test_deserialize_server_name test_ctxt =
+  assert_equal (Some LockServ.Server) (LockServSerialization.deserializeName "Server")
+
+let test_deserialize_client_name test_ctxt =
+  assert_equal (Some (LockServ.Client 5)) (LockServSerialization.deserializeName "Client-5")
+
+let test_serialize_server_name test_ctxt =
+  assert_equal "Server" (LockServSerialization.serializeName LockServ.Server)
+
+let test_serialize_client_name test_ctxt =
+  assert_equal "Client-0" (LockServSerialization.serializeName (LockServ.Client 0))
+
+let test_list =
+  [
+    "deserialize server name", test_deserialize_server_name;
+    "deserialize client name", test_deserialize_client_name;
+    "serialize server name", test_serialize_server_name;
+    "serialize client name", test_serialize_client_name;
+  ]
+
+let tests =
+  "Serialization" >:::
+    (map test_list ~f:(fun (name, test_fn) ->
+      name >:: (fun test_ctxt ->
+	bracket ignore tear_down test_ctxt;
+	test_fn test_ctxt)
+     ))
